src/Parsers/BooleanRecognizerOptimized.v
@@ -8,6 +8,7 @@ Require Import ADTSynthesis.Parsers.StringLike.Properties.
 Require Import ADTSynthesis.Common ADTSynthesis.Common.Wf.
 Require Import ADTSynthesis.Parsers.BooleanRecognizer.
 Require Import ADTSynthesis.Common.Match.
+Require Import ADTSynthesis.Common.List.ListFacts.
 Require Import ADTSynthesis.Common.Equality.
 Require Export ADTSynthesis.Common.SetoidInstances.
 
@@ -16,6 +17,44 @@ Local Open Scope string_like_scope.
 
 Global Arguments string_dec : simpl never.
 Global Arguments string_beq : simpl never.
+Global Arguments parse_production _ _ _ _ _ _ _ _ !_.
+
+Lemma parse_production_respectful {Char HSL HSLP predata A B}
+      {f g : forall (a : _ * A) (b : B a) (str : @String Char HSL), str ≤s (fst a) -> String.string -> bool}
+      (H : forall a b c d e, f a b c d e = g a b c d e)
+      str0 a b str pf
+: pointwise_relation
+    _ eq
+    (@parse_production Char HSL HSLP predata str0 (f (str0, a) b) str pf)
+    (@parse_production Char HSL HSLP predata str0 (g (str0, a) b) str pf).
+Proof.
+  intro ls.
+  revert str0 a b str pf; induction ls; simpl; trivial; intros.
+  setoid_rewrite IHls.
+  apply f_equal.
+  apply map_Proper_eq; trivial; repeat intro.
+  f_equal.
+  unfold parse_item.
+  destruct a; trivial.
+Qed.
+
+Ltac Fix3_setoid_rewrite H :=
+  etransitivity;
+  [ try clear H
+  | match goal with
+      | [ |- _ = @Fix3 ?A ?B ?C ?D ?R ?wf ?P ?f ?a ?b ?c ?d ]
+        => refine ((fun H => @Fix3_Proper_eq A B C D R wf P _ f H a b c d) _)
+    end;
+    unfold forall_relation, pointwise_relation, respectful;
+    let H' := fresh in
+    (intros ??? H' ???);
+      let L := match goal with |- ?L = _ => constr:L end in
+      let e := fresh "e" in
+      set (e := L);
+        setoid_rewrite <- (parse_production_respectful H');
+        setoid_rewrite H; try clear H;
+        subst e;
+        reflexivity ].
 
 Ltac extract_parser_opt :=
   eexists;
@@ -27,381 +66,49 @@ Ltac extract_parser_opt :=
   try unfold G';
     cbv beta iota zeta delta [parse_nonterminal parse_nonterminal_or_abort parse_nonterminal_step parse_productions parse_item Lookup list_to_grammar list_to_productions];
     simpl;
-    (let H0 := fresh "H0" in
-     (lazymatch goal with
-     | [ |- context[fold_right ?f ?i (map _ (bool_rect _ ?x ?y (string_beq ?s _)))] ]
-       => pose proof (fun g s' => @pull_bool_rect _ _ (fun ls => fold_right f i (map g ls)) x y (string_beq s s')) as H0;
-      simpl in H0
-      end);
-     etransitivity;
-     [ clear H0
-     | clear e;
+    repeat Fix3_setoid_rewrite (fun ls => eq_sym (@fold_symmetric _ orb Bool.orb_assoc Bool.orb_comm false ls));
+    repeat
+      (let H0 := fresh "H0" in
        match goal with
-         | [ |- _ = @Fix3 ?A ?B ?C ?D ?R ?wf ?P ?f ?a ?b ?c ?d ]
-           => refine ((fun H => @Fix3_Proper_eq A B C D R wf P _ f H a b c d) _)
+         | [ |- context[fold_right ?f ?i (map _ (bool_rect _ ?x ?y (string_beq ?s _)))] ]
+           => (pose proof (fun g s' => @pull_bool_rect _ _ (fun ls => fold_right f i (map g ls)) x y (string_beq s s')) as H0;
+               simpl in H0;
+               Fix3_setoid_rewrite H0)
+         | [ |- appcontext[fold_right (fun str_t else_case s => bool_rect (fun _ => ?T) (@?a str_t) (else_case s) (@?b str_t s))] ]
+           => (pose proof (@fold_right_fun _ _ _ (fun str_t else_cases s => bool_rect (fun _ => T) (a str_t) else_cases (b str_t s))) as H0;
+               simpl in H0;
+               Fix3_setoid_rewrite H0)
+         | [ |- context[@map _ ?B _ (fold_right (fun x acc => bool_rect (fun _ => _) (@?a x) acc _) ?init ?ls)] ]
+           => (pose proof (fun b' f => @f_fold_right_bool_rect _ (list B) _ (map f) init ls a b') as H0;
+               simpl in H0;
+               Fix3_setoid_rewrite H0)
+         | [ |- appcontext[?f (fold_right (fun x acc => bool_rect (fun _ => _) _ acc _) _ ?ls) ?x] ]
+           => (pose proof (fun init => @f_fold_right_bool_rect _ _ _ (fun k => f k x) init ls) as H0;
+               simpl in H0;
+               Fix3_setoid_rewrite H0)
+         | [ |- appcontext[?f (fold_right (fun x acc => bool_rect (fun _ => _) _ acc _) _ ?ls)] ]
+           => (pose proof (fun init => @f_fold_right_bool_rect _ _ _ f init ls) as H0;
+               simpl in H0;
+               Fix3_setoid_rewrite H0)
        end;
-       unfold forall_relation, pointwise_relation, respectful;
-       let H := fresh in
-       intros ??? H ???;
-              let L := match goal with |- ?L = _ => constr:L end in
-              let e := fresh "e" in
-              set (e := L);
-                setoid_rewrite H0; clear H0;
-                unfold parse_production, parse_item;
-                simpl;
-                setoid_rewrite <- H; subst e;
-                reflexivity
-     ]);
-    cbv beta iota zeta delta [sumbool_rect bool_rect];
+       instantiate;
+       simpl);
+    repeat Fix3_setoid_rewrite Bool.orb_false_r;
     subst e;
+    cbv beta iota zeta delta [bool_rect sumbool_rect];
     reflexivity.
 
-Require Import Grammars.ABStar.
-
 Section recursive_descent_parser.
-  Context {HSL : StringLike Ascii.ascii} {HSLP : StringLikeProperties Ascii.ascii}.
-  Context {data : @boolean_parser_dataT Ascii.ascii _}.
+  Context {Char} {HSL : StringLike Char} {HSLP : StringLikeProperties Char}
+          {ls : list (String.string * productions Char)}.
+  Context {data : @boolean_parser_dataT Char _}.
+  Local Notation G := (list_to_grammar (nil::nil) ls) (only parsing).
 
   Definition parse_nonterminal_opt
              (str : String)
              (nt : String.string)
-  : { b : bool | b = parse_nonterminal (G := ab_star_grammar) str nt }.
+  : { b : bool | b = parse_nonterminal (G := G) str nt }.
   Proof.
     extract_parser_opt.
   Defined.
-
-
-
-Focus 2.
-reflexivity.
-let H := fresh in
-intros
-  Focus 2.
-
-  setoid_rewrite <- H.
-  clear H y.
-
-
-  setoid_rewrite <- H.
-
-  let H0'
-
-  setoid_rewrite H0.
-
-Ltac pre_higher_order_reflexivity_one_evar :=
-  idtac;
-  match goal with
-    | [ |- ?l = ?r ]
-      => has_evar l; not has_evar r
-    | [ |- ?l = ?r ]
-      => has_evar r; not has_evar l; symmetry
-  end.
-
-Ltac higher_order_reflexivity_one_evar' :=
-  clear;
-  (lazymatch goal with
-  | [ |- ?f ?x = ?g ]
-    => revert x
-   end);
-  (lazymatch goal with
-  | [ |- forall x, ?f x = @?g x ]
-    => (let y := fresh in
-        intro y;
-        refine (@f_equal _ _ (fun f' => f' y) f g _))
-   end).
-
-Ltac higher_order_reflexivity_one_evar :=
-  pre_higher_order_reflexivity_one_evar;
-  repeat higher_order_reflexivity_one_evar'.
-
-{ higher_order_reflexivity_one_evar.
-  move a at bottom.
-  clear.
-  clear.
-
-  clear;
-  (lazymatch goal with
-  | [ |- ?f ?x = ?g ]
-    => revert x
-   end);
-  (lazymatch goal with
-  | [ |- forall x, ?f x = @?g x ]
-    => (let y := fresh in
-        intro y;
-        refine (@f_equal _ _ (fun f' => f' y) f g _))
-   end).
-
-
-  (lazymatch goal with
-  | [ |- ?f ?x = ?g ]
-    => revert x
-   end);
-  (lazymatch goal with
-  | [ |- forall x, ?f x = @?g x ]
-    => (let y := fresh in
-        intro y;
-        refine (@f_equal _ _ (fun f' => f' y) f g _))
-   end).
-  idtac;
-  (lazymatch goal with
-  | [ |- ?f ?x = ?g ]
-    => revert x
-   end);
-  (lazymatch goal with
-  | [ |- forall x, ?f x = @?g x ]
-    => intro x;
-   refine (@f_equal _ _ (fun f' => f' x) f g _)
-   end).
-(lazymatch goal with
-  | [ |- ?f ?x = ?g ]
-    => let g' := fresh "g'" in
-       set (g' := g);
-   pattern x in g';
-   subst g'
-   end);
-  (lazymatch goal with
-  | [ |- ?f ?x = ?g ?x ]
-    => refine (@f_equal _ _ (fun f' => f' x) f g _)
-   end).
-
-Lemma fg_equal_dep {A B} (f g : forall x : A, B x) (H : f = g)
-
-
-Ltac higher_order_5_reflexivity :=
-  let x := match goal with |- ?R ?x (?f ?a ?b ?c ?d ?e) => constr:(x) end in
-  let f := match goal with |- ?R ?x (?f ?a ?b ?c ?d ?e) => constr:(f) end in
-  let a := match goal with |- ?R ?x (?f ?a ?b ?c ?d ?e) => constr:(a) end in
-  let b := match goal with |- ?R ?x (?f ?a ?b ?c ?d ?e) => constr:(b) end in
-  let c := match goal with |- ?R ?x (?f ?a ?b ?c ?d ?e) => constr:(c) end in
-  let d := match goal with |- ?R ?x (?f ?a ?b ?c ?d ?e) => constr:(d) end in
-  let e := match goal with |- ?R ?x (?f ?a ?b ?c ?d ?e) => constr:(e) end in
-  let x' := (eval pattern a, b, c, d, e in x) in
-  let f' := match x' with ?f' _ _ _ _ _ => constr:(f') end in
-  unify f f';
-    cbv beta;
-    solve [apply reflexivity].
-
-Ltac higher_order_5_f_reflexivity :=
-  let x := match goal with |- ?R (?g ?x) (?g' (?f ?a ?b ?c ?d ?e)) => constr:(x) end in
-  let f := match goal with |- ?R (?g ?x) (?g' (?f ?a ?b ?c ?d ?e)) => constr:(f) end in
-  let a := match goal with |- ?R (?g ?x) (?g' (?f ?a ?b ?c ?d ?e)) => constr:(a) end in
-  let b := match goal with |- ?R (?g ?x) (?g' (?f ?a ?b ?c ?d ?e)) => constr:(b) end in
-  let c := match goal with |- ?R (?g ?x) (?g' (?f ?a ?b ?c ?d ?e)) => constr:(c) end in
-  let d := match goal with |- ?R (?g ?x) (?g' (?f ?a ?b ?c ?d ?e)) => constr:(d) end in
-  let e := match goal with |- ?R (?g ?x) (?g' (?f ?a ?b ?c ?d ?e)) => constr:(e) end in
-  let x' := (eval pattern a, b, c, d, e in x) in
-  let f' := match x' with ?f' _ _ _ _ _ => constr:(f') end in
-  unify f f';
-    cbv beta;
-    solve [apply reflexivity].
-let x := match goal with |- ?R ?x (?f ?a ?b ?c ?d ?e) => constr:(x) end in
-  let f := match goal with |- ?R ?x (?f ?a ?b ?c ?d ?e) => constr:(f) end in
-  let a := match goal with |- ?R ?x (?f ?a ?b ?c ?d ?e) => constr:(a) end in
-  let b := match goal with |- ?R ?x (?f ?a ?b ?c ?d ?e) => constr:(b) end in
-  let c := match goal with |- ?R ?x (?f ?a ?b ?c ?d ?e) => constr:(c) end in
-  let d := match goal with |- ?R ?x (?f ?a ?b ?c ?d ?e) => constr:(d) end in
-  let e := match goal with |- ?R ?x (?f ?a ?b ?c ?d ?e) => constr:(e) end in
-  let x' := (eval pattern e, d, b in x) in
-  idtac.
-  let f' := match x' with ?f' _ _ _ _ _ => constr:(f') end in
-  unify f f';
-    cbv beta;
-    solve [apply reflexivity].
-
-
-  higher_order_5_reflexivity.
-  higher_order_reflexivity.
-  Print Ltac higher_order_reflexivity.
-  higher_order_reflexivity.
-  reflexivity.
-      setoid_rewrite H0 ].
-  Focus 2.
-
-  reflexivity.
-  Focus 2.
-Require Import Ascii.
-Delimit Scope char_scope with char.
-  setoid_rewrite H.
-
-
-
-  setoid_rewrite
-
-specialize (H0 X).
-  refine (Fix3_Proper_eq _ _ _ _ _ _ _).
-  appyl
-    Typeclasses eauto := debug.
-    try timeout 1 setoid_rewrite H.
-    match goal with
-    eexists; simpl.
-    reflexivity.
-  Defined.
-End recursive_descent_parser.
-
-Require Import Grammars.ABStar.
-Require Import StringLike.String.
-Require Import Splitters.RDPList.
-Section recursive_descent_parser'.
-  Definition parse_nonterminal_opt' d : _ -> _ -> bool := fun str nt => proj1_sig (@parse_nonterminal_opt _ string_stringlike string_stringlike_properties ab_star_grammar d str nt).
-  Locate string_dec.
-  Local Arguments String.string_dec : simpl never.
-  Goal True.
-    pose parse_nonterminal_opt' as b.
-    unfold parse_nonterminal_opt' in b.
-    unfold parse_nonterminal_opt in b.
-    Opaque parse_production.
-    simpl in b.
-
-  Context {Char} {HSL : StringLike Char} {HSLP : StringLikeProperties Char} {G : grammar Char}.
-  Context {data : @boolean_parser_dataT Char _}.
-
-    match goal with
-      | [ |-
-
-
-    unfold parse_nonterminal,
-    := @parse_nonterminal_or_abort
-         (str : String, initial_nonterminals_data) str
-         (or_intror (reflexivity _)) nt.
-
-
-
-  Section bool.
-    Section parts.
-      Definition parse_item
-                 (str_matches_nonterminal : String.string -> bool)
-                 (str : String)
-                 (it : item Char)
-      : bool
-        := match it with
-             | Terminal ch => str ~= [ ch ]
-             | NonTerminal nt => str_matches_nonterminal nt
-           end.
-
-      Section production.
-        Context {str0}
-                (parse_nonterminal
-                 : forall (str : String),
-                     str ≤s str0
-                     -> String.string
-                     -> bool).
-
-        (** To match a [production], we must match all of its items.
-            But we may do so on any particular split. *)
-        Fixpoint parse_production
-                 (str : String)
-                 (pf : str ≤s str0)
-                 (prod : production Char)
-        : bool.
-        Proof.
-          refine
-            match prod with
-              | nil =>
-                (** 0-length production, only accept empty *)
-                Nat.eq_dec (length str) 0
-              | it::its
-                => let parse_production' := fun str pf => parse_production str pf its in
-                   fold_right
-                     orb
-                     false
-                     (map (fun n =>
-                             (parse_item
-                                (parse_nonterminal (str := take n str) _)
-                                (take n str)
-                                it)
-                               && parse_production' (drop n str) _)%bool
-                          (split_string_for_production it its str))
-            end;
-          revert pf; clear -HSLP; intros;
-          abstract (rewrite ?str_le_take, ?str_le_drop; assumption).
-        Defined.
-      End production.
-
-      Section productions.
-        Context {str0}
-                (parse_nonterminal
-                 : forall (str : String)
-                          (pf : str ≤s str0),
-                     String.string -> bool).
-
-        (** To parse as a given list of [production]s, we must parse as one of the [production]s. *)
-        Definition parse_productions
-                   (str : String)
-                   (pf : str ≤s str0)
-                   (prods : productions Char)
-        : bool
-          := fold_right orb
-                        false
-                        (map (parse_production parse_nonterminal pf)
-                             prods).
-      End productions.
-
-
-      Section nonterminals.
-        Section step.
-          Context {str0 valid}
-                  (parse_nonterminal
-                   : forall (p : String * nonterminals_listT),
-                       prod_relation (ltof _ length) nonterminals_listT_R p (str0, valid)
-                       -> forall str : String,
-                            str ≤s fst p -> String.string -> bool).
-
-          Definition parse_nonterminal_step
-                     (str : String)
-                     (pf : str ≤s str0)
-                     (nt : String.string)
-          : bool.
-          Proof.
-            refine
-              (if lt_dec (length str) (length str0)
-               then (** [str] got smaller, so we reset the valid nonterminals list *)
-                 parse_productions
-                   (@parse_nonterminal
-                      (str : String, initial_nonterminals_data)
-                      (or_introl _))
-                   (or_intror (reflexivity _))
-                   (Lookup G nt)
-               else (** [str] didn't get smaller, so we cache the fact that we've hit this nonterminal already *)
-                 if Sumbool.sumbool_of_bool (is_valid_nonterminal valid nt)
-                 then (** It was valid, so we can remove it *)
-                   parse_productions
-                     (@parse_nonterminal
-                        (str0 : String, remove_nonterminal valid nt)
-                        (or_intror (conj eq_refl (remove_nonterminal_dec _ nt _))))
-                     (str := str)
-                     _
-                     (Lookup G nt)
-                 else (** oops, we already saw this nonterminal in the past.  ABORT! *)
-                   false);
-            assumption.
-          Defined.
-        End step.
-
-        Section wf.
-          (** TODO: add comment explaining signature *)
-          Definition parse_nonterminal_or_abort
-          : forall (p : String * nonterminals_listT)
-                   (str : String),
-              str ≤s fst p
-              -> String.string
-              -> bool
-            := Fix3
-                 _ _ _
-                 (well_founded_prod_relation
-                    (well_founded_ltof _ length)
-                    ntl_wf)
-                 _
-                 (fun sl => @parse_nonterminal_step (fst sl) (snd sl)).
-
-          Definition parse_nonterminal
-                     (str : String)
-                     (nt : String.string)
-          : bool
-            := @parse_nonterminal_or_abort
-                 (str : String, initial_nonterminals_data) str
-                 (or_intror (reflexivity _)) nt.
-        End wf.
-      End nonterminals.
-    End parts.
-  End bool.
 End recursive_descent_parser.
