src/Parsers/ParserFromParserADT.v
@@ -1,7 +1,8 @@
 (** Reference implementation of a splitter and parser based on that splitter *)
 Require Import Coq.Strings.String.
 Require Import ADTSynthesis.Parsers.SplitterFromParserADT.
-Require Import ADTSynthesis.Parsers.ParserImplementation.
+Require Import ADTSynthesis.Parsers.ContextFreeGrammarNotations.
+Require Export ADTSynthesis.Parsers.ParserImplementationOptimized.
 Require Import ADTSynthesis.ADT.ComputationalADT.
 Require Import ADTSynthesis.ADTRefinement.GeneralRefinements.
 Require Import ADTSynthesis.Parsers.ParserADTSpecification.
@@ -18,11 +19,9 @@ Local Open Scope ADT_scope.
 Local Open Scope string_scope.
 
 Section parser.
-  Context (G : grammar Ascii.ascii).
+  Context {ls : list (String.string * productions Ascii.ascii)}.
+  Local Notation G := (list_to_grammar (nil::nil) ls) (only parsing).
   Context (splitter_impl : FullySharpened (string_spec G)).
-
-  Definition base_parser : Parser G (adt_based_splitter splitter_impl)
-    := parser (adt_based_splitter splitter_impl).
 
   Definition new_string_of_base_string (str : String.string)
     := (cConstructors (projT1 splitter_impl) {| StringBound.bindex := "new" |} (str : String.string)).
@@ -46,85 +45,22 @@ Section parser.
              str
              new_string_of_base_string_R)).
 
-  Definition soundness_type := forall str : @String _ string_stringlike,
-                                 has_parse base_parser (new_string_of_string str) = true ->
-                                 parse_of_item G str (NonTerminal G).
-
-  Definition string_has_parse (str : String.string) : bool
-    := has_parse
-         base_parser
-         (exist
-            _  (new_string_of_base_string str)
-            (ex_intro _ str new_string_of_base_string_R)).
-(*
-  Lemma string_parser_sound
-  : soundness_type.
+  Definition parser : Parser G string_stringlike.
   Proof.
-    Set Printing All.
-    Timeout 2 abstract (exfalso; admit).
-    admit.
-
-
-  Definition string_parser : Parser G string_stringlike.
-  Proof.
-    refine {| has_parse str
-              := has_parse
-                   base_parser
-                   (exist
-                      _  (new_string_of_base_string str)
-                      (ex_intro _ str new_string_of_base_string_R));
-              has_parse_sound := _;
-              has_parse_complete := _ |}.
-    { refine (fun str Hparse
-              => @transfer_parse_of_item
-                   Ascii.ascii (adt_based_StringLike splitter_impl) string_stringlike G
-                   (fun x y => AbsR (projT2 splitter_impl) y (` x))
-                   _ _ _ _ _ _ _ _ (has_parse_sound base_parser _ Hparse)).
-      admit.
-      { intros ????.
-        simpl.
-        erewrite mis_char_eq; intros; eassumption. }
-      { intros ???.
-        admit; erewrite mlength_eq; intros; eassumption. }
-    { intros; apply mtake_R; assumption. }
-    { intros; refine (mdrop_R _ _); assumption. }
-    { apply new_string_of_base_string_R. }
-  Qed.
-  Next Obligation.
-    refine (@transfer_parse_of_item Ascii.ascii (adt_based_StringLike splitter_impl) string_stringlike G
-                                    ((fun x y => AbsR (projT2 splitter_impl) y (` x)) : _ -> String.string -> Prop)
-                                    _ _ _ _ _ _ _ _ (has_parse_sound base_parser _ Hparse));
-    simpl.
-    { intros ????.
-      erewrite mis_char_eq; intros; eassumption. }
-    { intros ???.
-      erewrite mlength_eq; intros; eassumption. }
-    { intros; apply mtake_R; assumption. }
-    { intros; refine (mdrop_R _ _); assumption. }
-    { apply new_string_of_base_string_R. }
-  Qed.
-
-
-              (fun x (y : String.string) => AbsR (projT2 splitter_impl) x y)).
-    Focus 5.
-    pose .
-
-
-    dependent destruction p.
-    pose proof (@parse_nonterminal_complete Char splitter _ G _ _ rdp_list_rdata' str (Start_symbol G) p) as H'.
-    apply H'.
-    rewrite <- (parse_of_item_respectful_refl (pf := reflexivity _)).
-    rewrite <- (parse_of_item_respectful_refl (pf := reflexivity _)) in Hp.
-    eapply expand_forall_parse_of_item; [ | reflexivity.. | eassumption ].
-    simpl.
-    unfold rdp_list_is_valid_nonterminal; simpl.
-    intros ? ? ? ? ? H0.
-    edestruct List.in_dec as [ | nH ]; trivial; [].
-    destruct (nH H0).
-  Qed.
-
-
-
-
-*)
+    refine (@parser ls (adt_based_splitter splitter_impl)
+                    new_string_of_string
+                    (fun rep str => AbsR (projT2 splitter_impl) str (` rep))
+                    (@new_string_of_base_string_R) _ _);
+    abstract (
+        split;
+        first [ (intros ????);
+                simpl;
+                erewrite mis_char_eq; intros; eassumption
+              | (intros ???);
+                simpl;
+                erewrite mlength_eq; intros; eassumption
+              | intros; apply mtake_R; assumption
+              | intros; refine (mdrop_R _ _); assumption ]
+      ).
+  Defined.
 End parser.
