src/Parsers/ContextFreeGrammarTransferProperties.v
@@ -1,0 +1,85 @@
+(** * Properties about Context Free Grammars *)
+Require Import Coq.Numbers.Natural.Peano.NPeano.
+Require Import ADTSynthesis.Parsers.StringLike ADTSynthesis.Parsers.ContextFreeGrammar.
+Require Import Coq.Classes.RelationClasses.
+Require Import ADTSynthesis.Common ADTSynthesis.Common.UIP.
+Require Import ADTSynthesis.Parsers.ContextFreeGrammarProperties ADTSynthesis.Parsers.ContextFreeGrammarTransfer.
+
+Set Implicit Arguments.
+
+Local Open Scope list_scope.
+
+Section cfg.
+  Context {Char} {HSL1 HSL2 : StringLike Char}
+          {G : grammar Char}
+          {R : @String Char HSL1 -> @String Char HSL2 -> Prop}
+          {TR : transfer_respectful R}.
+  Context {P : String.string -> Type}.
+
+  Definition transfer_forall_parse_of_item'
+        (transfer_forall_parse_of
+         : forall str1 str2 it (HR : R str1 str2) p,
+             @Forall_parse_of Char _ G (fun _ => P) str1 it p
+             -> @Forall_parse_of Char _ G (fun _ => P) str2 it (transfer_parse_of HR p))
+        {str1 str2 it}
+        (HR : R str1 str2)
+        {p}
+  : @Forall_parse_of_item' Char HSL1 G (fun _ => P) (@Forall_parse_of _ _ _ (fun _ => P)) str1 it p
+    -> @Forall_parse_of_item' Char HSL2 G (fun _ => P) (@Forall_parse_of _ _ _ (fun _ => P)) str2 it (transfer_parse_of_item HR p)
+    := match
+        p in (parse_of_item _ _ it)
+        return
+        (@Forall_parse_of_item' Char HSL1 G (fun _ => P) (@Forall_parse_of _ _ _ (fun _ => P)) str1 it p
+         -> @Forall_parse_of_item' Char HSL2 G (fun _ => P) (@Forall_parse_of _ _ _ (fun _ => P)) str2 it (transfer_parse_of_item HR p))
+      with
+        | ParseTerminal _ _ => fun x => x
+        | ParseNonTerminal _ p' => fun xy => (fst xy, transfer_forall_parse_of _ _ _ _ p' (snd xy))
+      end.
+
+  Fixpoint transfer_forall_parse_of
+           str1 str2 pats
+           (HR : R str1 str2)
+           {p}
+           {struct p}
+  : @Forall_parse_of Char HSL1 G (fun _ => P) str1 pats p
+    -> @Forall_parse_of Char HSL2 G (fun _ => P) str2 pats (transfer_parse_of HR p)
+    := match
+        p in (parse_of _ _ pats)
+        return
+        (@Forall_parse_of Char HSL1 G (fun _ => P) str1 pats p
+         -> @Forall_parse_of Char HSL2 G (fun _ => P) str2 pats (transfer_parse_of HR p))
+      with
+        | ParseHead _ _ p' => @transfer_forall_parse_of_production _ _ _ _ p'
+        | ParseTail _ _ p' => @transfer_forall_parse_of _ _ _ _ p'
+      end
+  with transfer_forall_parse_of_production
+         str1 str2 pat
+         (HR : R str1 str2)
+         {p}
+         {struct p}
+       : @Forall_parse_of_production Char HSL1 G (fun _ => P) str1 pat p
+         -> @Forall_parse_of_production Char HSL2 G (fun _ => P) str2 pat (transfer_parse_of_production HR p)
+       := match
+           p in (parse_of_production _ _ pat)
+           return
+           (@Forall_parse_of_production Char HSL1 G (fun _ => P) str1 pat p
+            -> @Forall_parse_of_production Char HSL2 G (fun _ => P) str2 pat (transfer_parse_of_production HR p))
+         with
+           | ParseProductionNil _ => fun x => x
+           | ParseProductionCons _ _ _ p0 p1
+             => fun xy
+                => (@transfer_forall_parse_of_item' (@transfer_forall_parse_of) _ _ _ _ p0 (fst xy),
+                    @transfer_forall_parse_of_production _ _ _ _ p1 (snd xy))
+         end.
+
+  Global Arguments transfer_forall_parse_of {_ _ _} HR {_} _.
+  Global Arguments transfer_forall_parse_of_production {_ _ _} HR {_} _.
+
+  Definition transfer_forall_parse_of_item
+             {str1 str2 it}
+             (HR : R str1 str2)
+             {p}
+  : @Forall_parse_of_item Char HSL1 G (fun _ => P) str1 it p
+    -> @Forall_parse_of_item Char HSL2 G (fun _ => P) str2 it (transfer_parse_of_item HR p)
+    := @transfer_forall_parse_of_item' (@transfer_forall_parse_of) str1 str2 it HR p.
+End cfg.
