src/Parsers/ExtrOcamlParsers.v
@@ -1,0 +1,9 @@
+Require Import Coq.Arith.Compare_dec.
+Require Import ADTSynthesis.Common.Equality.
+Require Export ExtrOcamlBasic.
+Require Export ExtrOcamlNatInt.
+Require Export ExtrOcamlString.
+Extract Inlined Constant Compare_dec.lt_dec => "(<)".
+Extract Inlined Constant Sumbool.sumbool_of_bool => "(fun x -> x)".
+Extract Inlined Constant Equality.ascii_beq => "(=)".
+Extract Inlined Constant ascii_eq_dec => "(=)".
