src/Parsers/Refinement/SharpenedABStar.v
@@ -18,11 +18,13 @@ Section IndexedImpl.
 
     FullySharpenEachMethodWithoutDelegation.
     extract delegate-free implementation.
+    simpl; higher_order_reflexivityT.
   Defined.
 
 End IndexedImpl.
 
 Require Import ADTSynthesis.Parsers.ParserFromParserADT.
+Require Import ADTSynthesis.Parsers.ExtrOcamlParsers.
 
 Local Ltac do_compute_in term hyp :=
   let term' := (eval compute in term) in
@@ -36,8 +38,21 @@ Local Ltac do_simpl_in term hyp :=
   let term' := (eval simpl in term) in
   change term with term' in hyp.
 
+Local Ltac do_hnf_in term hyp :=
+  let term' := (eval hnf in term) in
+  change term with term' in hyp.
+
+Local Ltac set_subst_hnf_in term hyp :=
+  let H := fresh in
+  set (H := term) in hyp;
+    hnf in H;
+    cbv beta iota zeta delta [H] in hyp;
+    subst H.
+
 Local Arguments string_dec : simpl never.
 Local Arguments Equality.string_beq : simpl never.
+Arguments SplitterFromParserADT.msplits / .
+Arguments splits_for / .
 Local Notation hextr0 := (ex _).
 Local Notation exist' x := (exist _ x _).
 Local Notation hextr1 := (or_intror _).
@@ -45,8 +60,22 @@ Local Notation hextr2 := (or_introl _).
 
 Definition ab_star_parser' (str : String.string) : bool.
 Proof.
-  pose (string_has_parse ComputationalSplitter str) as impl.
-  cbv beta iota zeta delta [string_has_parse ParserInterface.has_parse base_parser ParserImplementation.parser BooleanRecognizer.parse_nonterminal BooleanRecognizer.parse_nonterminal_or_abort BooleanRecognizer.parse_nonterminal_step BooleanRecognizer.parse_productions BaseTypes.initial_nonterminals_data BooleanBaseTypes.predata ParserImplementation.parser_data RDPList.rdp_list_predata BaseTypes.remove_nonterminal BaseTypes.nonterminals_listT_R BaseTypes.nonterminals_listT RDPList.rdp_list_nonterminals_listT RDPList.rdp_list_nonterminals_listT_R BaseTypes.is_valid_nonterminal RDPList.rdp_list_is_valid_nonterminal BaseTypes.ntl_wf RDPList.rdp_list_remove_nonterminal] in impl.
+  pose (has_parse (parser ComputationalSplitter) str) as impl.
+  Timeout 2 cbv beta iota zeta delta [has_parse parser ParserImplementationOptimized.parser transfer_parser List.fold_right] in impl.
+  repeat (let impl' := (eval cbv delta [impl] in impl) in
+          match impl' with
+            | appcontext G[fst (?x, _)] => let G' := context G[x] in change impl' with G' in impl
+            | appcontext G[snd (_, ?x)] => let G' := context G[x] in change impl' with G' in impl
+          end).
+  Timeout 2 cbv beta iota zeta delta [List.map List.hd List.fold_left item_ascii_cons item_of_char item_of_string] in impl.
+  repeat (let impl' := (eval cbv delta [impl] in impl) in
+          match impl' with
+            | appcontext G[fst (?x, _)] => let G' := context G[x] in change impl' with G' in impl
+            | appcontext G[snd (_, ?x)] => let G' := context G[x] in change impl' with G' in impl
+          end).
+  Timeout 2 cbv beta iota zeta delta [BooleanRecognizer.parse_production BooleanRecognizer.parse_item BooleanBaseTypes.split_string_for_production parser_data ParserImplementation.parser_data new_string_of_string] in impl.
+  change (orb false) with (fun x : bool => x) in impl.
+  cbv beta in impl.
   change (@StringLike.String Ascii.ascii (ParserInterface.string_type
                                             (SplitterFromParserADT.adt_based_splitter
                                                ComputationalSplitter)))
@@ -60,6 +89,151 @@ Proof.
   Timeout 2 change (new_string_of_base_string ComputationalSplitter str)
   with (str, (0, String.length str)) in impl.
   Timeout 2 cbv beta iota zeta in impl.
+  Timeout 2 cbv beta iota zeta delta [splits_for] in impl.
+  Timeout 2 cbv beta iota zeta delta [is_char string_type splits_for SplitterFromParserADT.adt_based_splitter] in impl.
+  Timeout 2 cbv beta iota zeta delta [SplitterFromParserADT.msplits ComputationalADT.cMethods ComputationalADT.pcMethods] in impl.
+  Timeout 2 match eval cbv delta [impl] in impl with
+              | context[@projT2 ?A ?B (@projT1 ?C ?D ComputationalSplitter)]
+                => set_subst_hnf_in (@projT2 A B (@projT1 C D ComputationalSplitter)) impl
+            end.
+  Timeout 2 cbv beta iota zeta delta [BuildComputationalADT.getcMethDef BuildComputationalADT.cMethBody] in impl.
+(** HERE *)
+Locate StringBound.ith_Bounded.
+Print StringBound.ith_Bounded.
+Print StringBound.BoundedIndex.
+Print StringBound.IndexBound.
+
+  Timeout 2 let H := fresh in
+            set (H := (projT2 (projT1 ComputationalSplitter))) in impl;
+              hnf in H;
+              subst H.
+
+  let
+  Timeout 2 set_subst_hnf_in (projT2 (projT1 ComputationalSplitter)) impl.
+  hnf in X.
+  Timeout 2 subst X.
+  Opaque AbsR.
+  Timeout 2 pose (sf := (splits_for
+                         (SplitterFromParserADT.adt_based_splitter
+                            ComputationalSplitter))).
+  hnf in sf.
+  Set Printing Implicit.
+  Opaque StringLike.String SplitterFromParserADT.adt_based_StringLike AbsR.
+  Opaque ComputationalSplitter.
+  Timeout 2 simpl in impl.
+  Transparent SplitterFromParserADT.adt_based_StringLike.
+  Timeout 2 simpl in impl.
+  Arguments SplitterFromParserADT.mis_char / .
+  Timeout 2 simpl in impl.
+  Unset Printing Implicit.
+  Transparent ComputationalSplitter.
+  Arguments ComputationalADT.cMethodType / .
+  Arguments ComputationalADT.cMethods / .
+  Arguments If_Then_Else / .
+  repeat (let impl' := (eval cbv delta [impl] in impl) in
+          match impl' with
+            | appcontext G[ComputationalADT.cMethods
+                             (projT1 ComputationalSplitter)
+                             {| StringBound.bindex := "splits";
+                                StringBound.indexb := ?b |}]
+              => let m' := (eval simpl in (ComputationalADT.cMethods
+                                             (projT1 ComputationalSplitter)
+                                             {| StringBound.bindex := "splits";
+                                                StringBound.indexb := b |})) in
+                 change ((ComputationalADT.cMethods
+                            (projT1 ComputationalSplitter)
+                            {| StringBound.bindex := "splits";
+                               StringBound.indexb := b |}))
+                 with m' in impl
+          end).
+  Timeout 2 (repeat (let impl' := (eval cbv delta [impl] in impl) in
+          match impl' with
+            | appcontext G[ComputationalADT.cMethods
+                             (projT1 ComputationalSplitter)
+                             {| StringBound.bindex := "is_char";
+                                StringBound.indexb := ?b |}]
+              => let m' := (eval simpl in (ComputationalADT.cMethods
+                                             (projT1 ComputationalSplitter)
+                                             {| StringBound.bindex := "is_char";
+                                                StringBound.indexb := b |})) in
+                 change ((ComputationalADT.cMethods
+                            (projT1 ComputationalSplitter)
+                            {| StringBound.bindex := "is_char";
+                               StringBound.indexb := b |}))
+                 with m' in impl
+          end)).
+  Timeout 2 cbv beta iota zeta in impl.
+  Timeout 2 (do 6 let impl' := (eval cbv delta [impl] in impl) in
+                    match impl' with
+                      | appcontext G[fst (?x, ?y)] => change (fst (x, y)) with x in impl
+                      | appcontext G[snd (?x, ?y)] => change (snd (x, y)) with y in impl
+                    end).
+  Opaque ComputationalSplitter.
+  Timeout 2 simpl in impl.
+  Timeout 5 (let impl' := (eval cbv delta [impl] in impl) in
+          match impl' with
+            | appcontext G[fst (?x, _)] => let G' := context G[x] in pose G'
+            | appcontext G[snd (_, ?x)] => let G' := context G[x] in change impl' with G' in impl
+          end).
+  Timeout 5 (let impl' := (eval cbv delta [impl] in impl) in
+                    match impl' with
+                      | appcontext G[fst (?x, ?y)] => timeout 2 change (fst (x, y)) with x in impl
+                      | appcontext G[snd (?x, ?y)] => timeout 2 change (snd (x, y)) with y in impl
+                    end).
+
+  Timeout 2 simpl in c.
+               | appcontext G[snd (_, ?x)] => let G' := context G[x] in change impl' with G' in impl
+             end).
+
+  match
+  Timeout 4 do_simpl_in (projT1 ComputationalSplitter) impl.
+  Arguments SplitterFromParserADT.mis_char / .
+    change (splits_for
+                         (SplitterFromParserADT.adt_based_splitter
+                            ComputationalSplitter)) with sf in impl.
+
+  Timeout 2 simpl in impl.
+  Timeout 2 cbv beta iota zeta delta [List.map] in impl.
+
+  Timeout 2 hnf in sf.
+  let T := match type of sf with ?T -> _ => constr:T end in
+  set (T' := T) in sf;
+    change T with T' in sf.
+  match eval cbv delta [sf] in sf with
+    | fun x : ?T => _ => change T with T' in sf
+  end.
+  Timeout 2 simpl in sf.
+  Timeout 2 cbv delta [sf] in impl.
+  subst T' sf.
+  Timeout 2 change
+  Timeout 2 simpl in sf.
+  Timeout 2 let term := constr:() in
+  let term' := (eval simpl in term) in
+  let term'' := (eval cbv beta in (fun str : { r : (String.string * (nat * nat)) | exists orig, AbsR (projT2 ComputationalSplitter) orig r }%type => term' str)) in
+  idtac.
+  change term with term'' in impl.
+  change term with
+Local Ltac do_simpl_in term hyp :=
+  let term' := (eval simpl in term) in
+  change term with term' in hyp.
+
+  Timeout 2 do_simpl_in () impl.
+assert (x : { r : (String.string * (nat * nat)) | exists orig, AbsR (projT2 ComputationalSplitter) orig r }%type) by (exfalso; clear; admit).
+pose (splits_for
+                                              (SplitterFromParserADT.adt_based_splitter
+                                                 ComputationalSplitter) x).
+Timeout 2 simpl in l.
+
+Timeout 2 simpl in l.
+
+  Timeout 2 simpl @fst in impl.
+
+  match goal with
+    | [
+  Timeout 2 unfold List.fold_right in impl.
+  Timeout 2 unfold BooleanRecognizer.parse_production in impl.
+  Timeout 2 simpl BooleanRecognizer.parse_production in impl.
+  cbv beta iota zeta delta [string_has_parse ParserInterface.has_parse base_parser ParserImplementation.parser BooleanRecognizer.parse_nonterminal BooleanRecognizer.parse_nonterminal_or_abort BooleanRecognizer.parse_nonterminal_step BooleanRecognizer.parse_productions BaseTypes.initial_nonterminals_data BooleanBaseTypes.predata ParserImplementation.parser_data RDPList.rdp_list_predata BaseTypes.remove_nonterminal BaseTypes.nonterminals_listT_R BaseTypes.nonterminals_listT RDPList.rdp_list_nonterminals_listT RDPList.rdp_list_nonterminals_listT_R BaseTypes.is_valid_nonterminal RDPList.rdp_list_is_valid_nonterminal BaseTypes.ntl_wf RDPList.rdp_list_remove_nonterminal] in impl.
   Timeout 2 do_simpl_in (Lookup ab_star_grammar) impl.
   Timeout 2 cbv beta iota zeta in impl.
   let impl' := (eval cbv delta [impl] in impl) in exact impl'.
